WIP

src/example/SpinLock.v
@@ -78,6 +78,207 @@ Liveness chain of a spinlock :
    *)
 
   (** Invariants. *)
+  Definition spinlockInv (n : nat) (r : nat) (x : SCMem.val) (P : Formula (1+n)) (k l : nat) : Formula (1+n) :=
+    ((∃ (q : τ{Qp, 1+n}),
+         (➢(auex_b_Qp q))
+           ∗
+           (((x ↦ 0) ∗ ◇[k](l + 1, 1) ∗ ➢(excls r) ∗ ➢(auex_w_Qp q) ∗ P)
+            ∨ ((x ↦ 1) ∗ live[k] q ∗ ∃ (u : τ{nat, 1+n}), live[u] (1/2) ∗ (-[u](0)-◇ emp) ∗ (u -(0)-◇ k))))
+     ∨ dead[k]
+    )%F.
+
+  Definition isSpinlock n (E : coPset) (r : nat) (x : SCMem.val) (P : Formula (1+n)) (k L l : nat) : Formula (1+n) :=
+    (∃ (N : τ{namespace, 1+n}),
+        ⌜(↑N ⊆ E)⌝ ∗ ◆[k, L] ∗ (⌜0 < l⌝) ∗ syn_inv _ N (spinlockInv n r x P k l))%F.
+
+
+  (* Lemma Spinlock_lock_spec *)
+  (*       tid n *)
+  (*       (Es : coPsets) (E : coPset) *)
+  (*       (MASK_TOP : OwnEs_top Es) *)
+  (*       (MASK_STTGT : mask_has_st_tgt Es n) *)
+  (*       (MASK_DISJ : E ## ↑N_state_tgt) *)
+  (*   : *)
+  (*   ⊢ *)
+  (*     ∀ r x (P : Formula (1+n)) k L l q (ds : list (nat * nat * Formula (1+n))), *)
+  (*       [@ tid, (2+n), Es @] *)
+  (*         ⧼(⟦(⤉((syn_tgt_interp_as n sndl (fun m => (➢ (scm_memory_black m)))) *)
+  (*               ∗ (isSpinlock n E r x P k L l) *)
+  (*                     ∗ live[k] q ∗ Duty(tid) ds ∗ ◇{List.map fst ds}(L, 2)))%F, 2+n⟧)⧽ *)
+  (*           (OMod.close_itree Client (SCMem.mod gvs) (Spinlock.lock Client x)) *)
+  (*           ⧼rv, (⟦(⤉(∃ (u : τ{nat, 1+n}), *)
+  (*                      ➢(excls r) ∗ P ∗ ➢(auex_w_Qp q) ∗ *)
+  (*                       Duty(tid) ((u, 0, emp) :: ds) ∗ ◇[u](l, 1)))%F , 2+n⟧)⧽ *)
+  (* . *)
+  Lemma Spinlock_lock_syn_spec
+        tid n
+        (Es : coPsets) (E : coPset)
+        (MASK_TOP : OwnEs_top Es)
+        (MASK_STTGT : mask_has_st_tgt Es n)
+        (MASK_DISJ : E ## ↑N_state_tgt)
+    :
+    ⊢ ⟦(∀ (r : τ{nat})
+          (x : τ{SCMem.val})
+          (P : τ{Φ, 2+n})
+          (k L l : τ{nat})
+          (q : τ{Qp})
+          (ds : τ{ listT (nat * nat * Φ)%ftype, 2+n}),
+        [@ tid, (1+n), Es @]
+          ⧼(((syn_tgt_interp_as n sndl (fun m => (➢ (scm_memory_black m))))
+                ∗ (isSpinlock n E r x P k L l)
+                      ∗ live[k] q ∗ Duty(tid) ds ∗ ◇{List.map fst ds}(L, 2)) : Formula (1+n))⧽
+            (OMod.close_itree Client (SCMem.mod gvs) (Spinlock.lock Client x))
+            ⧼rv, (∃ (u : τ{nat, 1+n}),
+                       ➢(excls r) ∗ (P) ∗ ➢(auex_w_Qp q) ∗
+                        Duty(tid) ((u, 0, emp) :: ds) ∗ ◇[u](l, 1))⧽)%F, 2+n⟧
+  .
+  Proof.
+    simpl.
+    red_tl. iIntros (r).
+    red_tl. iIntros (x).
+    red_tl. iIntros (P).
+    red_tl. iIntros (k).
+    red_tl. iIntros (L).
+    red_tl. iIntros (l).
+    red_tl. iIntros (q).
+    red_tl. iIntros (ds).
+    rewrite red_syn_non_atomic_triple. simpl in *.
+    (* iIntros (? ? ? ? ? ? ? ?). *)
+    iStartTriple. iIntros "PRE POST".
+    unfold Spinlock.lock.
+    (* Preprocess for induction. *)
+    iApply wpsim_free_all. auto.
+    unfold isSpinlock. ss.
+    iEval (red_tl; simpl) in "PRE". iEval (rewrite red_syn_tgt_interp_as) in "PRE".
+    iDestruct "PRE" as "(#STINTP & (%N & SL) & LIVE & DUTY & PCS)".
+    iEval (red_tl; simpl) in "SL". iDestruct "SL" as "(%IN & #LO & %POS & INV)".
+    iEval (rewrite red_syn_inv) in "INV". iPoseProof "INV" as "#INV".
+    iMod ((pcs_decr _ _ 1 1 2) with "PCS") as "[PCS PCS2]". ss.
+    iMod (ccs_make k L _ 0 with "[PCS2]") as "CCS". iFrame. auto.
+    iMod (pcs_drop _ _ _ _ 0 with "PCS") as "PCS". lia.
+    (* Set up induction hypothesis. *)
+    iRevert "LIVE DUTY PCS POST". iMod (ccs_ind with "CCS []") as "IND".
+    2:{ iApply "IND". }
+    iModIntro. iExists 0. iIntros "IH". iModIntro. iIntros "LIVE DUTY PCS POST".
+    (* Start an iteration. *)
+    iEval (rewrite unfold_iter_eq). rred2r.
+    iApply (wpsim_yieldR with "[DUTY PCS]").
+    2:{ iSplitL "DUTY". iApply "DUTY". iFrame. }
+
+    TODO
+
+    auto. Unshelve. 2: auto.
+    iIntros "DUTY FC". iModIntro. rred2r.
+    (* Case analysis on lock variable. *)
+    iInv "INV" as "SLI" "SLI_CLOSE". iEval (unfold spinlockInv; simpl; red_tl; simpl) in "SLI".
+    iDestruct "SLI" as "[[%q0 SLI] | DEAD]".
+    2:{ iExFalso. iPoseProof (not_dead with "[LIVE DEAD]") as "%F". iFrame. auto. }
+    iEval (red_tl; simpl) in "SLI". iDestruct "SLI" as "[qISB [ACQ|WAIT]]".
+
+    (** Case 1. Acquire the lock. *)
+    { iClear "IH". iDestruct "ACQ" as "(PT & PCk & EXCL & qISW & PROP)".
+      iApply (SCMem_cas_fun_spec _ _ _ (S n) with "[PT]"). auto.
+      { unfold mask_has_st_tgt. rewrite lookup_insert. clear - MASK_DISJ IN. set_solver. }
+      { iFrame. iApply tgt_interp_as_equiv. 2: iApply "STINTP".
+        iIntros. iEval (simpl; red_tl; simpl). iSplit; iIntros "P".
+        - iFrame. ss.
+        - iDestruct "P" as "[MB _]". iFrame.
+      }
+      iIntros (b) "(%u & %RES & PT)". destruct (SCMem.val_eq_dec 0 0).
+      2:{ exfalso. ss. }
+      clear e. des. subst. rred2r. iApply wpsim_tauR. rred2r.
+      (* Close the invariant spinlockInv: *)
+      (* 1. Allocate new obligation: I will release the lock. *)
+      iMod (alloc_obligation (l + 1)) as "(%k1 & #LO1 & PC1 & LIVE1)".
+      (* 2. Preprocess. *)
+      iPoseProof (live_split _ (1/2)%Qp (1/2)%Qp with "[LIVE1]") as "[LIVE1 LIVE1']".
+      { iEval (rewrite Qp.half_half). iFrame. }
+      iMod (pc_drop _ l _ _ (1+1) _ with "PC1") as "PC1". auto. Unshelve. 2: lia.
+      iPoseProof (pc_split with "PC1") as "[PC1 PC_POST]".
+      iMod (pc_mon _ 1 _ (0+1) _ _ with "PC1") as "PC1". Unshelve.
+      2:{ apply layer_drop_eq; auto. }
+      iMod (duty_add _ _ _ _ _ 0 (emp%F : Formula n) with "[DUTY PC1] []") as "DUTY".
+      { iFrame. }
+      { iModIntro. iEval (ss; red_tl). auto. }
+      iPoseProof (duty_tpromise with "DUTY") as "#PROM1".
+      { simpl. left. auto. }
+      iMod (link_new k1 k (l+1) 0 with "[PCk]") as "#LINK1".
+      { iFrame. eauto. }
+      assert (AUTH: URA.updatable
+                      (Auth.black ((Excl.just q0) : Excl.t Qp) ⋅ Auth.white ((Excl.just q0) : Excl.t Qp))
+                      (Auth.black ((Some q) : Excl.t Qp) ⋅ Auth.white ((Some q) : Excl.t Qp))).
+      { apply Auth.auth_update. ii. des. split.
+        - ur. ss.
+        - ur in FRAME. ur. des_ifs.
+      }
+      iCombine "qISB qISW" as "qIS". iMod (OwnM_Upd AUTH with "qIS") as "[qISB qISW]". clear AUTH.
+      (* Now close with SLI_CLOSE. *)
+      iMod ("SLI_CLOSE" with "[LIVE PT LIVE1' qISB]") as "_".
+      { iEval (unfold spinlockInv; simpl; red_tl; simpl).
+        iLeft. iExists q. iEval (red_tl; simpl). iSplitL "qISB"; [iFrame|].
+        iRight. iFrame. iExists k1. iEval (red_tl; simpl). iFrame. auto.
+      }
+      (* Finish with POST. *)
+      iApply "POST". iEval (red_tl; simpl). iExists k1. iEval (red_tl; simpl).
+      iFrame.
+    }
+
+    (** Case 2. Miss the lock and loop. *)
+    { iDestruct "WAIT" as "(PT & LIVE_SL & %k_other & WAIT)".
+      iEval (simpl; red_tl; simpl) in "WAIT". iDestruct "WAIT" as "(LIVE_O & #OATH & #LINK)".
+      iApply (SCMem_cas_fun_spec _ _ _ n with "[PT]"). auto.
+      { unfold mask_has_st_tgt. rewrite lookup_insert. clear - MASK_DISJ IN. set_solver. }
+      { iFrame. iApply tgt_interp_as_equiv. 2: iApply "STINTP".
+        iIntros. iEval (simpl; red_tl; simpl). iSplit; iIntros "P".
+        - iFrame. ss.
+        - iDestruct "P" as "[MB _]". iFrame.
+      }
+      iIntros (b) "(%u & %RES & PT)". destruct (SCMem.val_eq_dec 1 0).
+      { exfalso. ss. }
+      clear n0. des. subst. rred2r. iApply wpsim_tauR. rred2r. iApply wpsim_tauR.
+      (* Get credits from IH and the invariant. *)
+      iMod (tpromise_progress with "[FC]") as "[PC | [DEAD _]]".
+      { iFrame. iApply "OATH". }
+      2:{ iExFalso. iPoseProof (not_dead with "[LIVE_O DEAD]") as "%FALSE". iFrame. auto. }
+      iMod (link_amplify with "[PC]") as "PC".
+      { iFrame. iApply "LINK". }
+      iMod ("IH" with "PC") as "[PCS IH]". auto.
+      (* Close the invariant spinlockInv. *)
+      iMod ("SLI_CLOSE" with "[qISB LIVE_SL LIVE_O PT]") as "_".
+      { iEval (unfold spinlockInv; simpl; red_tl; simpl).
+        iLeft. iExists q0. iEval (red_tl; simpl). iSplitL "qISB"; [iFrame|].
+        iRight. iFrame. iExists k_other. iEval (red_tl; simpl). iFrame. auto.
+      }
+      (* Finish with IH. *)
+      iApply wpsim_stutter_mon. i; eauto. instantiate (1:=pt). i; auto.
+      iApply ("IH" with "LIVE DUTY PCS POST").
+    }
+  Qed.
+
+
+  (* Lemma spinlock_lock_spec2 *)
+  (*       n *)
+  (*       tid R_src R_tgt (Q : R_src -> R_tgt -> iProp) R G ps pt itr_src ktr_tgt *)
+  (*       (* (TOP : OwnEs_top Es) *) *)
+  (*       (Es : coPsets) E *)
+  (*       (MASK : match Es !! n with Some E' => E ⊆ E' | None => True end) *)
+  (*   : *)
+  (*   ⊢ *)
+  (*   (∀ r x (P : Formula n) k l q (ds : list (nat * nat * Formula n)), *)
+  (*       (Duty(tid) ds =|S n|={Es, ∅}=∗ emp%I) *)
+  (*       → *)
+  (*         (⟦((isSpinlock n E r x P k l) ∗ live(k, q) ∗ Duty(tid) ds ∗ ◇[List.map fst ds @ l](2))%F, n⟧) *)
+  (*           -∗ *)
+  (*           ((⟦(∃ (u : τ{nat}), (➢(excls r)) ∗ (➢(agree_w_Qp q)) ∗ P ∗ Duty(tid) ((u, l, emp) :: ds) ∗ ◇(u @ l) 1)%F , n⟧) *)
+  (*              -∗ *)
+  (*              (wpsim (S n) tid ∅ R G Q ps true itr_src (ktr_tgt tt))) *)
+  (*           -∗ *)
+  (*           wpsim (S n) tid Es R G Q ps pt itr_src *)
+  (*           (map_event emb_spinlock (Spinlock.lock x) >>= ktr_tgt)). *)
+  (* Proof. *)
+  (*   iIntros (? ? ? ? ? ? ?) "CLOSE PRE POST". *)
+
+    (** Invariants. *)
   Definition spinlockInv (n : nat) (r : nat) (x : SCMem.val) (P : Formula n) (k l : nat) : Formula n :=
     ((∃ (q : τ{Qp}),
          (➢(auex_b_Qp q))
@@ -216,28 +417,5 @@ Liveness chain of a spinlock :
       iApply ("IH" with "LIVE DUTY PCS POST").
     }
   Qed.
-
-
-  (* Lemma spinlock_lock_spec2 *)
-  (*       n *)
-  (*       tid R_src R_tgt (Q : R_src -> R_tgt -> iProp) R G ps pt itr_src ktr_tgt *)
-  (*       (* (TOP : OwnEs_top Es) *) *)
-  (*       (Es : coPsets) E *)
-  (*       (MASK : match Es !! n with Some E' => E ⊆ E' | None => True end) *)
-  (*   : *)
-  (*   ⊢ *)
-  (*   (∀ r x (P : Formula n) k l q (ds : list (nat * nat * Formula n)), *)
-  (*       (Duty(tid) ds =|S n|={Es, ∅}=∗ emp%I) *)
-  (*       → *)
-  (*         (⟦((isSpinlock n E r x P k l) ∗ live(k, q) ∗ Duty(tid) ds ∗ ◇[List.map fst ds @ l](2))%F, n⟧) *)
-  (*           -∗ *)
-  (*           ((⟦(∃ (u : τ{nat}), (➢(excls r)) ∗ (➢(agree_w_Qp q)) ∗ P ∗ Duty(tid) ((u, l, emp) :: ds) ∗ ◇(u @ l) 1)%F , n⟧) *)
-  (*              -∗ *)
-  (*              (wpsim (S n) tid ∅ R G Q ps true itr_src (ktr_tgt tt))) *)
-  (*           -∗ *)
-  (*           wpsim (S n) tid Es R G Q ps pt itr_src *)
-  (*           (map_event emb_spinlock (Spinlock.lock x) >>= ktr_tgt)). *)
-  (* Proof. *)
-  (*   iIntros (? ? ? ? ? ? ?) "CLOSE PRE POST". *)
 
 End SIM.
